Fill the holes in efield_lemmas.

floyd/efield_lemmas.v
@@ -3,6 +3,7 @@ Require Import floyd.assert_lemmas.
 Require Import floyd.client_lemmas.
 Require Import floyd.nested_pred_lemmas.
 Require Import floyd.nested_field_lemmas.
+Require floyd.fieldlist. Import floyd.fieldlist.fieldlist.
 Local Open Scope logic.
 
 Inductive LLRR : Type :=
@@ -126,6 +127,7 @@ Section CENV.
 
 Context {cs: compspecs}.
 
+(* Null Empty Path situation *)
 Definition type_almost_match e t lr:=
   match typeof e, t, lr with
   | Tpointer t0 a0, Tarray t1 _ a1, RRRR => eqb_type (typeof e) (Tpointer t1 a1)
@@ -133,117 +135,67 @@ Definition type_almost_match e t lr:=
   | _, _, _ => false
   end.
 
-Fixpoint legal_nested_efield_rec t_root e (gfs: list gfield) (tts: list type) lr: bool :=
+(* Null Empty Path situation *)
+Definition type_almost_match' e t lr:=
+  match typeof e, t, lr with
+  | _, _, LLLL => eqb_type (typeof e) t
+  | _, _, _ => false
+  end.
+
+Fixpoint legal_nested_efield_rec t_root (gfs: list gfield) (tts: list type): bool :=
   match gfs, tts with
-  | nil, nil => type_almost_match e t_root lr
+  | nil, nil => true
   | nil, _ => false
   | _ , nil => false
-  | gf :: gfs0, t0 :: tts0 => 
-    match nested_field_rec t_root gfs with
-    | Some (_, ttt) => (legal_nested_efield_rec t_root e gfs0 tts0 lr && eqb_type ttt t0)%bool
-    | None => false
-    end
+  | gf :: gfs0, t0 :: tts0 => (legal_nested_efield_rec t_root gfs0 tts0 && eqb_type (nested_field_type2 t_root gfs) t0)%bool
   end.
 
 Definition legal_nested_efield t_root e gfs tts lr :=
-  match gfs, tts, lr with
-  | nil, nil, RRRR => false
-  | nil, nil, LLLL => eqb_type t_root (typeof e)
-  | nil, _, _ => false
-  | _ , nil, _ => false
-  | gf :: gfs0, t0 :: tts0, _ => 
-    match nested_field_rec t_root gfs with
-    | Some (_, ttt) => (legal_nested_efield_rec t_root e gfs0 tts0 lr && eqb_type ttt t0)%bool
-    | None => false
-    end
-  end.
+ (match gfs with
+  | nil => type_almost_match' e t_root lr
+  | _ => type_almost_match e t_root lr
+  end &&
+  legal_nested_efield_rec t_root gfs tts)%bool.
 
-(*
-Lemma legal_nested_efield_cons: forall env t_root gf gfs t tts ,
-  legal_nested_efield env t_root (gf :: gfs) (t :: tts) = true ->
-  legal_nested_efield env t_root gfs tts = true.
+Lemma legal_nested_efield_rec_cons: forall t_root gf gfs t tts,
+  legal_nested_efield_rec t_root (gf :: gfs) (t :: tts) = true ->
+  legal_nested_efield_rec t_root gfs tts = true.
 Proof.
-Opaque nested_field_rec.
   intros.
   simpl in H.
-  valid_nested_field_rec t_root (gf :: gfs) H.
-  solve_nested_field_rec_cons_eq_Some H0;
-  rewrite andb_true_iff in H;
+  rewrite andb_true_iff in H.
   tauto.
-Transparent nested_field_rec.
 Qed.
-*)
-(*
-Lemma legal_nested_efield_nested_field_rec_isSome: forall env t_root e gfs tts lr,
-  legal_nested_efield env t_root e gfs tts lr = true -> isSome (nested_field_rec t_root gfs).
+
+Lemma typeof_nested_efield': forall rho t_root e ef efs gf gfs t tts,
+  legal_nested_efield_rec t_root (gf :: gfs) (t :: tts) = true ->
+  efield_denote (ef :: efs) (gf :: gfs) rho |--
+    !! (nested_field_type2 t_root (gf :: gfs) =
+        typeof (nested_efield e (ef :: efs) (t :: tts))).
 Proof.
   intros.
-  destruct gfs.
-  + simpl; auto.
-Opaque nested_field_rec.
-  + simpl in H.
-    destruct tts; try solve [inversion H].
-    destruct (nested_field_rec t_root (g :: gfs)); [simpl; auto | inversion H].
-Transparent nested_field_rec.
+  simpl in H.
+  rewrite andb_true_iff in H; destruct H.
+  apply eqb_type_true in H0; subst.
+  destruct ef; apply prop_right; reflexivity.
 Qed.
-*)
-
 
 Lemma typeof_nested_efield: forall t_root e efs gfs tts lr,
   legal_nested_efield t_root e gfs tts lr = true ->
   efield_denote efs gfs |--
     !! (nested_field_type2 t_root gfs = typeof (nested_efield e efs tts)).
 Proof.
-intros.
-simpl. intro rho.
-revert t_root efs tts H; induction gfs; intros.
-*
-destruct tts; [ | inv H].
-destruct lr; try discriminate.
-apply eqb_type_true in H. subst.
-destruct efs; simpl; intros.
-apply prop_right; reflexivity.
-destruct e0; apply FF_left.
-*
-destruct efs as [| ef efs].
-destruct a; simpl; intros; apply FF_left.
-destruct tts; [inv H | ].
-simpl in H.
-destruct (nested_field_rec t_root gfs) as [[ofs t0]|] eqn:?; [ | discriminate].
-(* specialize (IHgfs t0 efs tts).*)
-destruct t0; try discriminate; destruct a; try discriminate.
-+
-rewrite andb_true_iff in H; destruct H.
-apply eqb_type_true in H0; subst; auto.
-destruct ef; simpl; try apply FF_left.
-normalize.
-destruct (typeof i0); try contradiction.
-unfold nested_field_type2.
-simpl.
-rewrite Heqo.
-apply prop_right; auto.
-+
-destruct (compute_in_members i0 (co_members (get_co i))) eqn:?; try discriminate.
-rewrite andb_true_iff in H; destruct H.
-apply eqb_type_true in H0; subst; auto.
-destruct ef; simpl; try apply FF_left.
-normalize.
-unfold nested_field_type2.
-simpl.
-rewrite Heqo.
-rewrite Heqb.
-apply prop_right; auto.
-+
-destruct (compute_in_members i0 (co_members (get_co i))) eqn:?; try discriminate.
-rewrite andb_true_iff in H; destruct H.
-apply eqb_type_true in H0; subst; auto.
-destruct ef; simpl; try apply FF_left.
-normalize.
-unfold nested_field_type2.
-simpl.
-rewrite Heqo.
-rewrite Heqb.
-apply prop_right; auto.
+  intros.
+  unfold legal_nested_efield in H.
+  rewrite andb_true_iff in H.
+  intro rho; simpl.
+  destruct H.
+  destruct gfs, efs, tts;
+  try solve [inversion H0 | simpl; normalize | destruct e0; simpl; normalize].
+  + destruct lr; try discriminate.
+    apply eqb_type_true in H; subst.
+    apply prop_right; reflexivity.
+  + apply typeof_nested_efield'; auto.
 Qed.
 
 Lemma offset_val_sem_add_pi: forall ofs t0 e rho i,
@@ -257,8 +209,8 @@ Proof.
 Qed.
 
 Lemma By_reference_eval_expr: forall Delta e rho,
-  access_mode (typeof (e)) = By_reference ->
-  typecheck_environ Delta rho ->
+  access_mode (typeof e) = By_reference ->
+  tc_environ Delta rho ->
   tc_lvalue Delta e rho |-- 
   !! (eval_expr e rho = eval_lvalue e rho).
 Proof.
@@ -270,141 +222,14 @@ Proof.
 Qed.
 
 Lemma By_reference_tc_expr: forall Delta e rho,
-  access_mode (typeof (e)) = By_reference ->
-  typecheck_environ Delta rho ->
+  access_mode (typeof e) = By_reference ->
+  tc_environ Delta rho ->
   tc_lvalue Delta e rho |--  tc_expr Delta e rho.
 Proof.
   intros.
   unfold tc_lvalue, tc_expr.
   destruct e; simpl in *; try apply @FF_left; rewrite H; auto.
 Qed.
-
-(*
-Lemma efield_denote_mut: forall P Q Delta env,
-  (forall t_root e efs gfs tts, P t_root e efs gfs tts |-- efield_denote Delta efs gfs) ->
-  (forall t_root e, P t_root e nil nil nil |-- Q t_root e nil nil nil) ->
-  (forall t_root e efs gfs tts ei i t0 t1 n a,
-     legal_nested_efield env t_root gfs tts = true ->
-     legal_nested_efield env t_root (ArraySubsc i :: gfs) (t0 :: tts) = true ->
-     nested_field_type2 t_root gfs = Tarray t1 n a ->
-     0 <= i < n ->
-     uncompomize env t1 = t0 ->
-     type_almost_match e t_root ->
-     P t_root e efs gfs tts |-- Q t_root e efs gfs tts ->
-     P t_root e (eArraySubsc ei :: efs) (ArraySubsc i :: gfs) (t0 :: tts) |--
-     Q t_root e (eArraySubsc ei :: efs) (ArraySubsc i :: gfs) (t0 :: tts)) ->
-  (forall t_root e efs gfs tts i t0 t1 i0 f a,
-     legal_nested_efield env t_root gfs tts = true ->
-     legal_nested_efield env t_root (StructField i :: gfs) (t0 :: tts) = true ->
-     nested_field_type2 t_root gfs = Tstruct i0 f a ->
-     field_type i f = Errors.OK t1 ->
-     uncompomize env t1 = t0 ->
-     type_almost_match e t_root ->
-     P t_root e efs gfs tts |-- Q t_root e efs gfs tts ->
-     P t_root e (eStructField i :: efs) (StructField i :: gfs) (t0 :: tts) |--
-     Q t_root e (eStructField i :: efs) (StructField i :: gfs) (t0 :: tts)) ->
-  (forall t_root e efs gfs tts i t0 t1 i0 f a,
-     legal_nested_efield env t_root gfs tts = true ->
-     legal_nested_efield env t_root (UnionField i :: gfs) (t0 :: tts) = true ->
-     nested_field_type2 t_root gfs = Tunion i0 f a ->
-     field_type i f = Errors.OK t1 ->
-     uncompomize env t1 = t0 ->
-     type_almost_match e t_root ->
-     P t_root e efs gfs tts |-- Q t_root e efs gfs tts ->
-     P t_root e (eUnionField i :: efs) (UnionField i :: gfs) (t0 :: tts) |--
-     Q t_root e (eUnionField i :: efs) (UnionField i :: gfs) (t0 :: tts)) ->
-  forall t_root e efs gfs tts,
-  legal_nested_efield env t_root gfs tts = true ->
-   type_almost_match e t_root ->
-  P t_root e efs gfs tts |-- Q t_root e efs gfs tts.
-Proof.
-  intros.
-  revert gfs tts H4; induction efs as [| ef efs]; intros;
-  simpl; intro rho;
-  rewrite (add_andp _ _ (H _ _ _ _ _));
-  destruct gfs as [| gf gfs];
-  destruct tts as [| tt tts];
-  try solve [(simpl in H4; inversion H4)];
-  try solve [(simpl efield_denote; try destruct ef;
-              simpl; apply andp_left2; apply FF_left)].
-  + rewrite <- (add_andp _ _ (H _ _ _ _ _)); apply H0.
-  + pose proof legal_nested_efield_nested_field_rec_isSome _ _ _ _ H4.
-    destruct (nested_field_rec t_root (gf :: gfs)) as [[? ?]|] eqn: ?H;
-      [clear H6 | simpl in H6; inversion H6].
-    assert ((ef :: efs) <> nil) by (unfold not; intros ?H; congruence).
-    rewrite (add_andp _ _ (typeof_nested_efield _ _ _ _ _ _ _ H4 H6 H5)).
-    solve_nested_field_rec_cons_eq_Some H7; destruct ef;
-    try solve [(simpl efield_denote; try destruct ef;
-                simpl; apply andp_left2; apply andp_left1; apply FF_left)];
-    simpl efield_denote; normalize; apply andp_left1.
-Opaque nested_field_rec.
-    - unfold nested_field_type2 in H11; rewrite H7 in H11.
-      pose proof (legal_nested_efield_cons _ _ _ _ _ _ H4).
-      simpl in H1; eapply H1.
-      * exact H15.
-      * apply legal_nested_efield_cons in H4; rewrite H4.
-        rewrite H7, H11, eqb_type_refl.
-        reflexivity.
-      * unfold nested_field_type2.
-        rewrite H8; reflexivity.
-      * exact H9.
-      * exact H11.
-      * exact H5.
-      * apply IHefs.
-        eapply legal_nested_efield_cons, H4.
-    - unfold nested_field_type2 in H11; rewrite H7 in H11.
-      pose proof (legal_nested_efield_cons _ _ _ _ _ _ H4).
-      simpl in H2; eapply H2.
-      * exact H12.
-      * apply legal_nested_efield_cons in H4; rewrite H4.
-        rewrite H7, H11, eqb_type_refl.
-        reflexivity.
-      * unfold nested_field_type2.
-        rewrite H8; reflexivity.
-      * exact H9.
-      * exact H11.
-      * exact H5.
-      * apply IHefs.
-        eapply legal_nested_efield_cons, H4.
-    - unfold nested_field_type2 in H10; rewrite H7 in H10.
-      pose proof (legal_nested_efield_cons _ _ _ _ _ _ H4).
-      simpl in H3; eapply H3.
-      * exact H11.
-      * apply legal_nested_efield_cons in H4; rewrite H4.
-        rewrite H7, H10, eqb_type_refl.
-        reflexivity.
-      * unfold nested_field_type2.
-        rewrite H8; reflexivity.
-      * exact H9.
-      * exact H10.
-      * exact H5.
-      * apply IHefs.
-        eapply legal_nested_efield_cons, H4.
-Transparent nested_field_rec.
-Qed.
-*)
-
-Lemma classify_add_add_case_pi: forall ei t n a,
-  match typeof ei with | Tint _ _ _ => True | _ => False end ->
-  classify_add (Tarray t n a) (typeof ei) = add_case_pi t.
-Proof.
-  intros.
-  destruct (typeof ei); try solve [inversion H].
-  simpl.
-  destruct i; reflexivity.
-Qed.
-
-(*
-Lemma eval_lvalue_nested_efield_aux0: forall ei env Delta t_root e efs gfs tts t n a,
-  legal_nested_efield env t_root gfs tts = true ->
-  match typeof ei with | Tint _ _ _ => True | _ => False end ->
-  nested_field_type2 t_root gfs = Tarray t n a ->
-  type_almost_match e t_root ->
-  efield_denote Delta efs gfs |--
-  !! (classify_add (typeof (nested_efield e efs tts)) (typeof ei) = add_case_pi t).
-Proof.
-  Admitted.
-*)
 
 Definition eval_LR e lr :=
   match lr with
@@ -418,161 +243,343 @@ Definition tc_LR Delta e lr :=
   | RRRR => tc_expr Delta e
   end.
 
-Lemma eval_lvalue_nested_efield_aux: forall Delta t_root e efs gfs tts lr,
-  legal_nested_efield t_root e gfs tts lr = true ->
-  local (`isptr (eval_LR e lr)) &&  (tc_LR Delta e lr) &&
-     (tc_efield Delta efs) && efield_denote efs gfs |--
-  local (`isptr (eval_lvalue (nested_efield e efs tts))) &&
-     (tc_lvalue Delta (nested_efield e efs tts)) &&
-    local (`eq (eval_lvalue (nested_efield e efs tts))
-      (`(field_address t_root gfs) (eval_LR e lr))).
-Proof.
-Admitted.
-(*
-  intros.
-  apply efield_denote_mut 
-    with (P := fun t_root e efs gfs tts => local (`isptr (eval_lvalue e)) &&
-            local (tc_lvalue Delta e) && efield_denote Delta efs gfs)
-         (Q := fun t_root e efs gfs tts => local (`isptr (eval_lvalue (nested_efield e efs tts))) &&
-            local (tc_lvalue Delta (nested_efield e efs tts)) &&
-            local (`eq (eval_lvalue (nested_efield e efs tts))
-              (`(offset_val (Int.repr (nested_field_offset2 t_root gfs))) (eval_lvalue e))))
-         (Delta := Delta)
-         (env := env).
-  + intros. apply andp_left2; apply derives_refl.
-  + simpl; intros e0 rho. normalize.
-Opaque classify_add.
-  + (* Tarray *)
-    intros.
-    simpl; intro rho.
-    specialize (H7 rho).
-    unfold_lift.
-    normalize.
-    unfold_lift in H7.
-    normalize in H7.
-    rewrite (add_andp _ _ H7).
-    rewrite (add_andp _ _
-      (eval_lvalue_nested_efield_aux0 ei env Delta t_root0 e0 efs0 gfs0 tts0 t1 n a H1 H8 H3 H6)).
-    normalize.
-    apply prop_right.
-    unfold tc_lvalue.
-    simpl.
-    rewrite H16.
-    rewrite !denote_tc_assert_andp.
-    simpl.
-    unfold_lift.
-    admit.
-(*
-    assert (eval_expr (nested_efield e0 efs0 tts0) rho =
-            eval_lvalue (nested_efield e0 efs0 tts0) rho).
-      eapply By_reference_eval_expr. [rewrite <- H9; reflexivity | eauto]).
-    destruct (eval_lvalue (nested_efield e0 efs0 tts0) rho) eqn:?H; try inversion H10.
-    assert (offset_val Int.zero 
-           (force_val (sem_add (Tarray t1 n a) (typeof ei)
-           (eval_expr (nested_efield e0 efs0 tts0) rho) 
-           (eval_expr ei rho))) =
-           offset_val
-           (Int.repr (nested_field_offset2 (typeof e0) (ArraySubsc i :: gfs0)))
-           (eval_lvalue e0 rho) /\
-           isptr (force_val (sem_add (Tarray t1 n a) (typeof ei)
-           (eval_expr (nested_efield e0 efs0 tts0) rho) 
-           (eval_expr ei rho)))).
-    Focus 1. {
-      rewrite H15.
-      unfold sem_add.
-      rewrite classify_add_add_case_pi by exact H6.
-      rewrite <- H7, sem_add_pi_ptr by (simpl; auto).
-      simpl.
-      split; [| auto].
-      erewrite nested_field_offset2_Tarray by eauto.
-      destruct (eval_lvalue e0 rho); inversion H13.
-      simpl H12; inversion H12.
-      clear - H19.
-      simpl.
-      f_equal.
-      apply unsigned_eq_eq.
-      solve_mod_eq.
-      rewrite <- !Z.add_assoc.
-      solve_mod_eq.
-      rewrite !Z.add_assoc.
-      rewrite (Z.add_comm _ ((sizeof t1 * i) mod Int.modulus)).
-      rewrite <- Z.add_assoc.
-      solve_mod_eq.
-      f_equal.
-      change (Int.unsigned Int.zero) with 0.
-      omega.
-    } Unfocus.
-    destruct H17.
-    repeat split; auto.
-    - rewrite isptr_offset_val_zero by exact H18.
-      exact H18.
-    - rewrite H15; simpl; auto.
-    - apply By_reference_tc_expr.
-      rewrite <- H9; simpl; auto.
-      auto.
- *)
-  + (* Tstruct *)
-    intros.
-    simpl; intro rho.
-    simpl in H7; specialize (H7 rho).
-    rewrite andp_comm, !andp_assoc.
-    rewrite andp_comm in H7.
-    rewrite (add_andp _ _ H7).
-    admit.
-(*
-    rewrite (add_andp _ _ (typeof_nested_efield _ _ _ _ _ _ H0)).
-    normalize.
-    rewrite <- !prop_and; apply prop_right.
-    rewrite H2 in H6; simpl in H6.
-    rewrite <- H6.
-    unfold tc_lvalue.
-    simpl.
-    rewrite <- H6.
-    simpl.
-    rewrite denote_tc_assert_andp.
-    solve_field_offset_type i f; [| inversion H3].
-    repeat split; auto.
-    - destruct (eval_lvalue (nested_efield e0 efs0 tts0) rho); inversion H7.
-      simpl; auto.
-    - erewrite H9, nested_field_offset2_Tstruct by eauto.
-      destruct (eval_lvalue e0 rho); inversion H10.
-      simpl.
-      f_equal.
-      apply unsigned_eq_eq.
-      solve_mod_eq.
-      rewrite (Z.add_comm _ (nested_field_offset2 (typeof e0) gfs0 mod Int.modulus)).
-      rewrite <- Z.add_assoc.
-      solve_mod_eq.
-      f_equal; omega.
-*)
-  + (* Tunion *)
-    admit.
-  + exact H.
-  + exact H0.
-Qed.
-*)
-
-Lemma eval_lvalue_nested_efield: forall Delta t_root e efs gfs tts lr,
-  legal_nested_efield t_root e gfs tts lr = true ->
-  local (`isptr (eval_LR e lr)) &&  (tc_LR Delta e lr) &&
-   (tc_efield Delta efs) && efield_denote efs gfs |-- local (`eq (eval_lvalue (nested_efield e efs tts))
-      (`(field_address t_root gfs) (eval_LR e lr))).
+Lemma field_compatible_field_address: forall t gfs p, field_compatible t gfs p -> field_address t gfs p = offset_val (Int.repr (nested_field_offset2 t gfs)) p.
 Proof.
   intros.
-  eapply derives_trans; [eapply eval_lvalue_nested_efield_aux; eauto |].
-  simpl; intros; normalize. autorewrite with norm1 norm2; normalize.
+  unfold field_address.
+  rewrite if_true by auto.
+  auto.
 Qed.
 
-Lemma tc_lvalue_nested_efield: forall Delta t_root e efs gfs tts lr,
-  legal_nested_efield t_root e gfs tts lr = true ->
-  local (`isptr (eval_LR e lr)) &&  (tc_LR Delta e lr) &&
-   (tc_efield Delta efs) && efield_denote efs gfs |--
-    local (`isptr (eval_lvalue (nested_efield e efs tts))) &&
-     (tc_lvalue Delta (nested_efield e efs tts)).
+Definition LR_of_type (t: type) :=
+  match access_mode t with
+  | By_reference => RRRR
+  | _ => LLLL
+  end.
+
+Lemma legal_nested_efield_weaken: forall t_root e gfs tts,
+  legal_nested_efield t_root e gfs tts (LR_of_type t_root) = true ->
+  legal_nested_efield_rec t_root gfs tts = true /\
+  type_almost_match e t_root (LR_of_type t_root) = true.
 Proof.
   intros.
-  eapply derives_trans; [eapply eval_lvalue_nested_efield_aux; eauto |].
-  simpl; intros; normalize. autorewrite with norm1 norm2; normalize.
+  unfold legal_nested_efield in H.
+  rewrite andb_true_iff in H.
+  split; [tauto |].
+  destruct gfs; [| tauto].
+  destruct H as [? _].
+  unfold type_almost_match' in H.
+  unfold type_almost_match.
+  destruct (LR_of_type t_root), t_root, (typeof e); simpl in H |- *;
+  try inv H; auto.
+Qed.
+
+Lemma weakened_legal_nested_efield_spec: forall t_root e gfs efs tts rho,
+  legal_nested_efield_rec t_root gfs tts = true ->
+  type_almost_match e t_root (LR_of_type t_root) = true ->
+  efield_denote efs gfs rho
+       |-- !!(typeconv (nested_field_type2 t_root gfs) =
+              typeconv (typeof (nested_efield e efs tts))).
+Proof.
+  intros.
+  destruct gfs as [| [| |]], efs as [| [| |]], tts; try solve [inv H];
+  try solve [simpl; normalize];
+  try solve [rewrite (add_andp _ _ (typeof_nested_efield' _ t_root e _ _ _ _ _ _ H));
+             apply andp_left2; normalize; f_equal; auto].
+
+  apply prop_right.
+  rewrite nested_field_type2_ind.
+  simpl typeof.
+  unfold type_almost_match in H0.
+  destruct (LR_of_type t_root), t_root, (typeof e); try solve [inv H0]; auto;
+  apply eqb_type_spec in H0; rewrite H0; auto.
+Qed.
+
+Lemma classify_add_add_case_pi: forall ei ty t n a,
+  match typeof ei with | Tint _ _ _ => True | _ => False end ->
+  typeconv (Tarray t n a) = typeconv ty ->
+  classify_add ty (typeof ei) = add_case_pi t.
+Proof.
+  intros.
+  destruct (typeof ei); try solve [inversion H].
+  simpl.
+  rewrite <- H0.
+  destruct i; reflexivity.
+Qed.
+
+Lemma isBinOpResultType_add_ptr: forall e t n a t0 ei,
+  match typeof ei with | Tint _ _ _ => True | _ => False end ->
+  typeconv (Tarray t0 n a) = typeconv (typeof e) ->
+  complete_type cenv_cs t0 = true ->
+  isBinOpResultType Oadd e ei (tptr t) = tc_isptr e.
+Proof.
+  intros.
+  unfold isBinOpResultType.
+  erewrite classify_add_add_case_pi by eauto.
+  rewrite tc_andp_TT2.
+  rewrite H1, tc_andp_TT2.
+  auto.
+Qed.
+
+Lemma array_op_facts: forall ei rho t_root e efs gfs tts t n a t0 p,
+  legal_nested_efield_rec t_root gfs tts = true ->
+  type_almost_match e t_root (LR_of_type t_root) = true ->
+  match typeof ei with | Tint _ _ _ => True | _ => False end ->
+  nested_field_type2 t_root gfs = Tarray t n a ->
+  field_compatible t_root gfs p ->
+  complete_type cenv_cs t_root = true ->
+  efield_denote efs gfs rho =
+  efield_denote efs gfs rho &&
+  !! (classify_add (typeof (nested_efield e efs tts)) (typeof ei) = add_case_pi t /\
+      isBinOpResultType Oadd (nested_efield e efs tts) ei (tptr t0) = tc_isptr (nested_efield e efs tts)).
+Proof.
+  intros.
+  apply add_andp.
+  rewrite (add_andp _ _ (weakened_legal_nested_efield_spec _ _ _ _ _ _ H H0)); normalize.
+  apply prop_right.
+  rewrite H2 in H5.
+  split.
+  + eapply classify_add_add_case_pi; eauto.
+  + eapply isBinOpResultType_add_ptr; eauto.
+    eapply nested_field_type2_complete_type with (gfs0 := gfs) in H4; [| destruct H3; tauto].
+    rewrite H2 in H4.
+    exact H4.
+Qed.
+
+Lemma in_members_Ctypes_offset: forall i m e, in_members i m -> Ctypes.field_offset cenv_cs i m = Errors.Error e -> False.
+Proof.
+  intros.
+  unfold Ctypes.field_offset in H0.
+  revert H0; generalize 0; induction m as [| [? ?] ?]; intros.
+  + inv H.
+  + simpl in H0.
+    if_tac in H0; inv H0.
+    spec IHm.
+    - destruct H; [simpl in H; congruence | auto].
+    - apply IHm in H3; auto.
+Qed.
+
+Lemma struct_op_facts: forall Delta t_root e gfs efs tts i a i0 t rho,
+  legal_nested_efield_rec t_root gfs tts = true ->
+  legal_nested_field t_root (gfs DOT i0) ->
+  type_almost_match e t_root (LR_of_type t_root) = true ->
+  nested_field_type2 t_root gfs = Tstruct i a ->
+  efield_denote efs gfs rho =
+  efield_denote efs gfs rho &&
+  ((tc_lvalue Delta (nested_efield e efs tts) rho -->
+   tc_lvalue Delta (nested_efield e (eStructField i0 :: efs) (t :: tts)) rho) &&
+  !! (eval_field (typeof (nested_efield e efs tts)) i0 =
+      offset_val (Int.repr (field_offset cenv_cs i0 (co_members (get_co i)))))).
+Proof.
+  intros.
+  apply add_andp.
+  rewrite (add_andp _ _ (weakened_legal_nested_efield_spec _ _ _ _ _ _ H H1)); normalize.
+  rewrite H2 in H3; simpl in H3.
+  destruct (typeof (nested_efield e efs tts)) eqn:?H; inv H3.
+  1: destruct i1; inv H6.
+  destruct H0.
+  rewrite H2 in H3; simpl in H3.
+  unfold tc_lvalue, eval_field.
+  simpl.
+  rewrite H4.
+  unfold field_offset, fieldlist.field_offset2.
+  unfold get_co in *.
+  destruct (cenv_cs ! i1); [| inv H3].
+  destruct (Ctypes.field_offset cenv_cs i0 (co_members c)) eqn:?H.
+  + apply andp_right; normalize.
+    apply imp_andp_adjoint; apply andp_left2; auto.
+  + exfalso.
+    pose proof in_members_Ctypes_offset i0 (co_members c) e0; auto.
+Qed.
+
+Lemma union_op_facts: forall Delta t_root e gfs efs tts i a i0 t rho,
+  legal_nested_efield_rec t_root gfs tts = true ->
+  legal_nested_field t_root (gfs UDOT i0) ->
+  type_almost_match e t_root (LR_of_type t_root) = true ->
+  nested_field_type2 t_root gfs = Tunion i a ->
+  efield_denote efs gfs rho =
+  efield_denote efs gfs rho &&
+  ((tc_lvalue Delta (nested_efield e efs tts) rho -->
+   tc_lvalue Delta (nested_efield e (eUnionField i0 :: efs) (t :: tts)) rho) &&
+  !! (eval_field (typeof (nested_efield e efs tts)) i0 = offset_val Int.zero)).
+Proof.
+  intros.
+  apply add_andp.
+  rewrite (add_andp _ _ (weakened_legal_nested_efield_spec _ _ _ _ _ _ H H1)); normalize.
+  rewrite H2 in H3; simpl in H3.
+  destruct (typeof (nested_efield e efs tts)) eqn:?H; inv H3.
+  1: destruct i1; inv H6.
+  destruct H0.
+  rewrite H2 in H3; simpl in H3.
+  unfold tc_lvalue, eval_field.
+  simpl.
+  rewrite H4.
+  unfold get_co in *.
+  destruct (cenv_cs ! i1); [| inv H3].
+  apply andp_right; normalize.
+  apply imp_andp_adjoint; apply andp_left2; auto.
+Qed.
+
+Definition lvalue_LR_of_type: forall Delta rho P p t e,
+  P |-- !! (t = typeof e) ->
+  tc_environ Delta rho ->
+  P |-- !! (p = eval_lvalue e rho) && tc_lvalue Delta e rho ->
+  P |-- !! (p = eval_LR e (LR_of_type t) rho) && tc_LR Delta e (LR_of_type t) rho.
+Proof.
+  intros.
+  destruct (LR_of_type t) eqn:?H.
+  + exact H1.
+  + rewrite (add_andp _ _ H); clear H.
+    rewrite (add_andp _ _ H1); clear H1.
+    simpl; normalize.
+    apply andp_left2.
+    unfold LR_of_type in H2.
+    destruct (access_mode (typeof e)) eqn:?H; inv H2.
+    apply andp_right.
+    - eapply derives_trans; [apply By_reference_eval_expr |]; auto.
+      normalize.
+    - apply By_reference_tc_expr; auto.
+Qed.
+
+Lemma eval_lvalue_nested_efield_aux: forall Delta t_root e efs gfs tts p,
+  field_compatible t_root gfs p ->
+  legal_nested_efield t_root e gfs tts (LR_of_type t_root) = true ->
+  local (`(eq p) (eval_LR e (LR_of_type t_root))) &&
+  tc_LR Delta e (LR_of_type t_root) &&
+  local (tc_environ Delta) &&
+  tc_efield Delta efs &&
+  efield_denote efs gfs |--
+  local (`(eq (field_address t_root gfs p))
+   (eval_LR (nested_efield e efs tts) (LR_of_type (nested_field_type2 t_root gfs)))) &&
+  tc_LR Delta (nested_efield e efs tts) (LR_of_type (nested_field_type2 t_root gfs)).
+Proof.
+  intros.
+  unfold local, lift1; simpl; intro rho.
+  unfold_lift.
+  normalize.
+  apply legal_nested_efield_weaken in H0; destruct H0.
+  rewrite field_compatible_field_address by auto.
+  revert gfs tts H H0; induction efs as [| [| |]]; intros; destruct gfs as [| [| |]], tts;
+  try solve [inversion H0];
+  try solve [unfold efield_denote; normalize];
+  specialize (IHefs gfs tts);
+  (pose proof H;
+   apply field_compatible_cons in H;
+    destruct (nested_field_type2 t_root gfs) eqn:?H; try solve [inv H]);
+  pose proof (proj1 (proj1 (andb_true_iff _ _) H0) : legal_nested_efield_rec t_root gfs tts = true);
+  (spec IHefs; [tauto |]);
+  (spec IHefs; [auto |]);
+  (apply lvalue_LR_of_type;
+   [apply andp_left2; apply typeof_nested_efield'; auto | assumption |]).
+  + destruct H.
+    unfold tc_lvalue.
+    Opaque isBinOpResultType. simpl. Transparent isBinOpResultType.
+    unfold local, lift1; unfold_lift.
+    normalize.
+    erewrite array_op_facts with (t0 := t) by eauto; normalize.
+    rewrite !andp_assoc, (andp_comm (tc_expr Delta i rho)), <- !andp_assoc.
+    eapply derives_trans; [apply andp_derives; [exact IHefs | apply derives_refl] |].
+    normalize.
+    rewrite !denote_tc_assert_andp, H10.
+    unfold denote_tc_assert at 1 4, denote_tc_isptr; simpl.
+    unfold local, lift1, force_val2; unfold_lift.
+    assert (offset_val (Int.repr (nested_field_offset2 t_root (gfs SUB i0)))
+            (eval_LR e (LR_of_type t_root) rho) =
+            force_val
+               (sem_add (typeof (nested_efield e efs tts)) 
+                  (typeof i) (eval_expr (nested_efield e efs tts) rho)
+                  (eval_expr i rho)));
+     [| repeat apply andp_right; try apply prop_right; auto].
+    - rewrite offset_val_nested_field_offset2_ind by auto.
+      simpl; unfold sem_add.
+      unfold local, lift1; unfold_lift.
+      rewrite H9.
+      simpl in H11; rewrite <- H11, <- H7.
+      unfold force_val; rewrite sem_add_pi_ptr by auto.
+      f_equal.
+      rewrite mul_repr.
+      f_equal.
+      rewrite H4.
+      reflexivity.
+    - rewrite <- H12, isptr_offset_val_zero; auto.
+    - simpl in H11; rewrite <- H11; auto.
+    - apply andp_left1; auto.
+    - apply andp_left2; auto.
+    - rewrite <- H12; auto.
+  + destruct H.
+    simpl.
+    unfold local, lift1; unfold_lift.
+    normalize.
+    erewrite struct_op_facts with (Delta := Delta) (t := t) by eauto.
+    normalize.
+    rewrite <- !andp_assoc.
+    eapply derives_trans; [apply andp_derives; [apply IHefs | apply derives_refl] |]; normalize.
+    simpl.
+    eapply derives_trans; [apply modus_ponens |].
+    apply andp_right; [apply prop_right | auto].
+    rewrite H7.
+    rewrite offset_val_nested_field_offset2_ind by auto.
+    rewrite H4; simpl.
+    simpl in H8; rewrite <- H8.
+    reflexivity.
+  + destruct H.
+    simpl.
+    unfold local, lift1; unfold_lift.
+    normalize.
+    erewrite union_op_facts with (Delta := Delta) (t := t) by eauto.
+    normalize.
+    rewrite <- !andp_assoc.
+    eapply derives_trans; [apply andp_derives; [apply IHefs | apply derives_refl] |]; normalize.
+    simpl.
+    eapply derives_trans; [apply modus_ponens |].
+    apply andp_right; [apply prop_right | auto].
+    rewrite H7.
+    rewrite offset_val_nested_field_offset2_ind by auto.
+    rewrite H4; simpl.
+    simpl in H8; rewrite <- H8.
+    reflexivity.
+Qed.
+
+Lemma eval_lvalue_nested_efield: forall Delta t_root e efs gfs tts lr p,
+  field_compatible t_root gfs p ->
+  LR_of_type t_root = lr ->
+  legal_nested_efield t_root e gfs tts lr = true ->
+  type_is_by_value (nested_field_type2 t_root gfs) = true ->
+  local (`(eq p) (eval_LR e lr)) &&
+  tc_LR Delta e lr &&
+  local (tc_environ Delta) &&
+  tc_efield Delta efs &&
+  efield_denote efs gfs |--
+  local (`(eq (field_address t_root gfs p)) (eval_lvalue (nested_efield e efs tts))).
+Proof.
+  intros.
+  subst lr.
+  eapply derives_trans; [apply eval_lvalue_nested_efield_aux; eauto |].
+  apply andp_left1.
+  destruct (LR_of_type (nested_field_type2 t_root gfs)) eqn:?H; auto.
+  unfold LR_of_type in H0.
+  destruct (nested_field_type2 t_root gfs) as [| [| | |] [|] | | [|] | | | | |]; inv H2; inv H0.
+Qed.
+
+Lemma tc_lvalue_nested_efield: forall Delta t_root e efs gfs tts lr p,
+  field_compatible t_root gfs p ->
+  LR_of_type t_root = lr ->
+  legal_nested_efield t_root e gfs tts lr = true ->
+  type_is_by_value (nested_field_type2 t_root gfs) = true ->
+  local (`(eq p) (eval_LR e lr)) &&
+  tc_LR Delta e lr &&
+  local (tc_environ Delta) &&
+  tc_efield Delta efs &&
+  efield_denote efs gfs |--
+  tc_lvalue Delta (nested_efield e efs tts).
+Proof.
+  intros.
+  subst lr.
+  eapply derives_trans; [apply eval_lvalue_nested_efield_aux; eauto |].
+  apply andp_left2.
+  destruct (LR_of_type (nested_field_type2 t_root gfs)) eqn:?H; auto.
+  unfold LR_of_type in H0.
+  destruct (nested_field_type2 t_root gfs) as [| [| | |] [|] | | [|] | | | | |]; inv H2; inv H0.
 Qed.
 
 End CENV.
